src/rocq/Handlers/Handlers.v
@@ -18,6 +18,7 @@
    [bind], [vis] and [trigger], as well as the proof that they respect [eutt].
  *)
 
+Unset Universe Checking.
 From Vellvm.Handlers Require Export
      Global
      Local
