src/rocq/Handlers/SerializationTheory.v
@@ -3,7 +3,7 @@ From Stdlib Require Import ZArith Lia List String.
 From ExtLib Require Import
      Core.RelDec
      Structures.Monads.
-
+Unset Universe Checking.
 From Vellvm Require Import
      Utils.Util
      Utils.Tactics
