src/rocq/Semantics/InterpretationStack.v
@@ -8,6 +8,7 @@ From ITree Require Import
 From ITreeSpec Require Import
   ITreeSpecDefinition.
 
+Unset Universe Checking.
 From Vellvm Require Import
      Utilities
      Semantics.LLVMEvents
@@ -74,9 +75,13 @@ Module Type InterpreterStack_common (LP : LLVMParams) (MEM : Memory LP).
       let L2_trace       := interp_local_stack L1_trace l in
       L2_trace.
 
-    Definition interp_mcfg3 {R} (RR : Relation_Definitions.relation (@stack_frame uvalue local_env * @stack uvalue local_env * (global_env * R)))  (t: itree L0 R) (g : global_env) (l : @stack_frame uvalue local_env * @stack uvalue local_env) (sid : store_id) (m : MemState) : PropT L3 (MemState * (store_id * (@stack_frame uvalue local_env * @stack uvalue local_env * (global_env * R)))) :=
+    Definition interp_mcfg3 {R} (RR : Relation_Definitions.relation (@stack_frame uvalue local_env * @stack uvalue local_env * (global_env * R)))
+                                (t: itree L0 R) 
+                                (g : global_env) 
+                                (l : @stack_frame uvalue local_env * @stack uvalue local_env) 
+                                (sid : store_id) (m : MemState) : itree_spec L3 (MemState * (store_id * (@stack_frame uvalue local_env * @stack uvalue local_env * (global_env * R)))) :=
       let L2_trace       := interp_mcfg2 t g l in
-      let L3_trace       := interp_memory_spec RR L2_trace sid m in
+      let L3_trace       := interp_memory_spec L2_trace sid m in
       L3_trace.
 
     Definition interp_mcfg3_exec {R} (t: itree L0 R) g l sid m : itree L3 (MemState * (store_id * (@stack_frame uvalue local_env * @stack uvalue local_env * (global_env * R)))) :=
@@ -84,7 +89,7 @@ Module Type InterpreterStack_common (LP : LLVMParams) (MEM : Memory LP).
       let L3_trace       := interp_memory L2_trace sid m in
       L3_trace.
 
-    Definition interp_mcfg4 {R} RR_mem RR_pick (t: itree L0 R) g l sid m : PropT L4 (MemState * (store_id * (@stack_frame uvalue local_env * @stack uvalue local_env * (global_env * R)))) :=
+    Definition interp_mcfg4 {R} RR_mem RR_pick (t: itree L0 R) g l sid m : itree_spec L4 (MemState * (store_id * (@stack_frame uvalue local_env * @stack uvalue local_env * (global_env * R)))) :=
       let L3_trace       := interp_mcfg3 RR_mem t g l sid m in
       let L4_trace       := model_undef RR_pick L3_trace in
       L4_trace.
@@ -94,7 +99,7 @@ Module Type InterpreterStack_common (LP : LLVMParams) (MEM : Memory LP).
       let L4_trace       := exec_undef L3_trace in
       L4_trace.
 
-    Definition interp_mcfg5 {R} RR_mem RR_pick (t: itree L0 R) g l sid m : PropT L5 (MemState * (store_id * (@stack_frame uvalue local_env * @stack uvalue local_env * (global_env * R)))) :=
+    Definition interp_mcfg5 {R} RR_mem RR_pick (t: itree L0 R) g l sid m : itree_spec L5 (MemState * (store_id * (@stack_frame uvalue local_env * @stack uvalue local_env * (global_env * R)))) :=
       let L4_trace       := interp_mcfg4 RR_mem RR_pick t g l sid m in
       let L5_trace       := model_UB L4_trace in
       L5_trace.
