src/rocq/Theory/StatePredicates.v
@@ -1,4 +1,5 @@
 (* begin hide *)
+Unset Universe Checking.
 From Vellvm Require Import
      Semantics.LLVMParams
      Semantics.Lang.
